Lean4Lean/Tests.lean
@@ -8,6 +8,8 @@ import Lean4Lean.Tests.Toolchain
 import Lean4Lean.Tests.ConditionReflect
 import Lean4Lean.Tests.ModDivCondition
 import Lean4Lean.Tests.NatDiv
+import Lean4Lean.Tests.NatGcd
+import Lean4Lean.Tests.NatGcdProdState
 import Lean4Lean.Tests.NatMod
 import Lean4Lean.Tests.DifferentialParity
 import Lean4Lean.Tests.Environment
